figured out a way to formalize specs and morhpisms without signatures

Base.v
@@ -15,36 +15,22 @@ Require Import Util.
  ** The basic structures: signatures, models, and specs
  **)
 
-(* A signature is a glorified record type *)
-Inductive Sig : list string -> Type :=
-| Sig_Nil : Sig nil
-| Sig_Cons f (A : Type) flds : (A -> Sig flds) -> Sig (f :: flds)
-.
-
-(* FIXME: previous version with a requirement of uniqueness of fields *)
-(*
-Inductive Sig : list string -> Type :=
-| Sig_Nil : Sig nil
-| Sig_Cons f (A : Type) flds : ~In f flds -> (A -> Sig flds) -> Sig (f :: flds)
-.
-*)
-
 (* A Model is an element of the record type denoted by a Sig *)
-Inductive Model : forall {flds}, Sig flds -> Type :=
-| Model_Nil : Model Sig_Nil
-| Model_Cons f A a flds sig  :
-    Model (flds:=flds) (sig a) ->
-    Model (Sig_Cons f A flds sig)
+Inductive Model : forall {flds : list string}, Type :=
+| Model_Nil : Model (flds:=nil)
+| Model_Cons f A (a : A) flds :
+    Model (flds:=flds) ->
+    Model (flds:= f :: flds)
 .
 
 (* A Spec is a partial Model of a Sig *)
-Inductive Spec : forall {flds}, Sig flds -> Type :=
-| Spec_Nil : Spec Sig_Nil
-| Spec_ConsNone f A flds sig  :
-    (forall a, Spec (flds:=flds) (sig a)) -> Spec (Sig_Cons f A flds sig)
-| Spec_ConsSome f A a flds sig  :
-    Spec (flds:=flds) (sig a) ->
-    Spec (Sig_Cons f A flds sig)
+Inductive Spec : forall {flds : list string}, Type :=
+| Spec_Nil : Spec (flds:=nil)
+| Spec_ConsNone f A flds :
+    (forall (a:A), Spec (flds:=flds)) -> Spec (flds:= f :: flds)
+| Spec_ConsSome f A (a : A) flds :
+    Spec (flds:=flds) ->
+    Spec (flds:= f :: flds)
 .
 
 
@@ -52,43 +38,23 @@ Inductive Spec : forall {flds}, Sig flds -> Type :=
  ** Notions of elements of structures
  **)
 
-(* FIXME: don't think I really need SigElem... *)
-(* Proof that field f is associated with type A in signature, where A
-   quantifies over all types before f in the Sig *)
-Inductive SigElem (f : string) : Type -> forall {flds}, Sig flds -> Prop :=
-| SigElem_Base A flds sig :
-    SigElem f A (Sig_Cons f A flds sig)
-| SigElem_Cons f' A' A flds sig :
-    (forall (a:A'), SigElem f (A a) (sig a)) ->
-    SigElem f (forall (a:A'), A a) (Sig_Cons f' A' flds sig)
-.
-
-(* Proof that field f is associated with non-dependent type A in signature *)
-Inductive SigElem_nondep (f : string) A : forall {flds}, Sig flds -> Prop :=
-| SigElem_nondep_Base flds sig :
-    SigElem_nondep f A (Sig_Cons f A flds sig)
-| SigElem_nondep_Cons f' A' flds sig :
-    (forall a, SigElem_nondep f A (sig a)) ->
-    SigElem_nondep f A (Sig_Cons f' A' flds sig)
-.
-
 (* Proof that field f is associated with element a of type A in model *)
-Inductive ModelElem (f : string) A (a:A) : forall {flds sig}, Model (flds:=flds) sig -> Prop :=
-| ModelElem_Base flds sig model :
-    ModelElem f A a (Model_Cons f A a flds sig model)
-| ModelElem_Cons f' A' a' flds sig model :
+Inductive ModelElem (f : string) A (a:A) : forall {flds}, Model (flds:=flds) -> Prop :=
+| ModelElem_Base flds model :
+    ModelElem f A a (Model_Cons f A a flds model)
+| ModelElem_Cons f' A' a' flds model :
     ModelElem f A a model ->
-    ModelElem f A a (Model_Cons f' A' a' flds sig model)
+    ModelElem f A a (Model_Cons f' A' a' flds model)
 .
 
 (* Projecting an element out of a Model *)
-Fixpoint modelProj {flds sig} (model : Model (flds:=flds) sig) :
+Fixpoint modelProj {flds} (model : Model (flds:=flds)) :
   forall f, In f flds -> { A : Type & A } :=
-  match model in Model (flds:=flds) sig
+  match model in Model (flds:=flds)
         return forall f, In f flds -> { A : Type & A }
   with
     | Model_Nil => fun f in_nil => False_rect _ in_nil
-    | Model_Cons f' A a _ _ model =>
+    | Model_Cons f' A a _ model =>
       fun f in_pf =>
         match string_dec f' f with
             | left _ => existT id A a
@@ -98,13 +64,13 @@ Fixpoint modelProj {flds sig} (model : Model (flds:=flds) sig) :
   end.
 
 (* Correctness of modelProj: always returns a ModelElem *)
-Lemma modelProj_correct flds sig (model : Model (flds:=flds) sig) f in_pf :
+Lemma modelProj_correct flds (model : Model (flds:=flds)) f in_pf :
   ModelElem f (projT1 (modelProj model f in_pf))
             (projT2 (modelProj model f in_pf))
             model.
   revert f in_pf; induction model; intros.
   elimtype False; apply in_pf.
-  unfold modelProj; fold (modelProj (flds:=flds) (sig:=sig a)).
+  unfold modelProj; fold (modelProj (flds:=flds)).
   destruct (string_dec f f0).
   rewrite <- e; apply ModelElem_Base.
   apply ModelElem_Cons.
@@ -119,35 +85,16 @@ Qed.
 (* A model of a Spec supplies missing fields but is otherwise equal;
    this definition requires the signatures of spec and model to be
    definitionally equal, and so is homogeneous *)
-Inductive IsModel_hom : forall {flds sig}, Spec (flds:=flds) sig -> Model (flds:=flds) sig -> Prop :=
-| IsModel_hom_Nil : IsModel_hom Spec_Nil Model_Nil
-| IsModel_hom_ConsNone f A a flds sig spec model :
-    IsModel_hom (spec a) model ->
-    IsModel_hom (Spec_ConsNone f A flds sig spec)
-            (Model_Cons f A a flds sig model)
-| IsModel_hom_ConsSome f A a flds sig spec model :
-    IsModel_hom spec model ->
-    IsModel_hom (Spec_ConsSome f A a flds sig spec)
-            (Model_Cons f A a flds sig model)
-.
-
-(* A model of a Spec supplies missing fields but is otherwise equal;
-   this definition allows the signatures of spec and model to be
-   provably, instead of definitionally, equal, and so is
-   heterogeneous, similar to heterogeneous (John-Major) equality *)
-Inductive IsModel_het :
-  forall {flds sig_s},
-    Spec (flds:=flds) sig_s ->
-    forall {sig_m}, Model (flds:=flds) sig_m -> Prop :=
-| IsModel_het_Nil : IsModel_het Spec_Nil Model_Nil
-| IsModel_het_ConsNone f A a flds sig spec model :
-    IsModel_het (spec a) model ->
-    IsModel_het (Spec_ConsNone f A flds sig spec)
-            (Model_Cons f A a flds sig model)
-| IsModel_het_ConsSome f A a flds sig spec model :
-    IsModel_het spec model ->
-    IsModel_het (Spec_ConsSome f A a flds sig spec)
-            (Model_Cons f A a flds sig model)
+Inductive IsModel : forall {flds}, Spec (flds:=flds) -> Model (flds:=flds) -> Prop :=
+| IsModel_Nil : IsModel Spec_Nil Model_Nil
+| IsModel_ConsNone f A a flds spec model :
+    IsModel (spec a) model ->
+    IsModel (Spec_ConsNone f A flds spec)
+            (Model_Cons f A a flds model)
+| IsModel_ConsSome f A a flds spec model :
+    IsModel spec model ->
+    IsModel (Spec_ConsSome f A a flds spec)
+            (Model_Cons f A a flds model)
 .
 
 (* FIXME: write prove_ismodel tactic *)
@@ -156,17 +103,17 @@ Inductive IsModel_het :
  ** Oooh, supermodels!
  **)
 
-Fixpoint SuperModel {flds1 sig1} (model1 : Model (flds:=flds1) sig1)
-         {flds2 sig2} (model2 : Model (flds:=flds2) sig2) : Prop :=
+Fixpoint SuperModel {flds1} (model1 : Model (flds:=flds1))
+         {flds2} (model2 : Model (flds:=flds2)) : Prop :=
   match model2 with
     | Model_Nil => True
-    | Model_Cons f A a flds2' sig2' model2' =>
+    | Model_Cons f A a flds2' model2' =>
       ModelElem f A a model1 /\ SuperModel model1 model2'
   end.
 
-Lemma SuperModel_cons_l f A a {flds1 sig1} model1 {flds2 sig2} model2 :
-  SuperModel model1 (flds2:=flds2) (sig2:=sig2) model2 ->
-  SuperModel (Model_Cons f A a flds1 sig1 model1) model2.
+Lemma SuperModel_cons_l f A a {flds1} model1 {flds2} model2 :
+  SuperModel model1 (flds2:=flds2) model2 ->
+  SuperModel (Model_Cons f A a flds1 model1) model2.
   induction model2.
   intro; apply I.
   intro H; apply conj.
@@ -174,8 +121,8 @@ Lemma SuperModel_cons_l f A a {flds1 sig1} model1 {flds2 sig2} model2 :
   apply IHmodel2; destruct H; assumption.
 Qed.
 
-Lemma SuperModel_id {flds sig} model :
-  SuperModel (flds1:=flds) (sig1:=sig) model model.
+Lemma SuperModel_id {flds} model :
+  SuperModel (flds1:=flds) model model.
   induction model.
   apply I.
   apply conj;
@@ -183,23 +130,23 @@ Lemma SuperModel_id {flds sig} model :
     | apply SuperModel_cons_l; assumption ].
 Qed.
 
-Lemma SuperModel_elem {flds2 sig2} (model2 : Model (flds:=flds2) sig2)
-      {flds1 sig1} (model1 : Model (flds:=flds1) sig1)
+Lemma SuperModel_elem {flds2} (model2 : Model (flds:=flds2))
+      {flds1} (model1 : Model (flds:=flds1))
       f A a (elem : ModelElem f A a model2) :
   SuperModel model1 model2 ->
   ModelElem f A a model1.
-  revert flds1 sig1 model1; induction elem; intros.
+  revert flds1 model1; induction elem; intros.
   destruct H; assumption.
   apply IHelem; destruct H; assumption.
 Qed.
 
-Lemma SuperModel_trans {flds1 sig1} (model1 : Model (flds:=flds1) sig1)
-      {flds2 sig2} (model2 : Model (flds:=flds2) sig2)
-      {flds3 sig3} (model3 : Model (flds:=flds3) sig3) :
+Lemma SuperModel_trans {flds1} (model1 : Model (flds:=flds1))
+      {flds2} (model2 : Model (flds:=flds2))
+      {flds3} (model3 : Model (flds:=flds3)) :
   SuperModel model1 model2 -> SuperModel model2 model3 ->
   SuperModel model1 model3.
   intros super12 super23;
-  revert flds1 sig1 model1 super12; induction model3; intros.
+  revert flds1 model1 super12; induction model3; intros.
   apply I.
   apply conj.
   destruct super23; apply (SuperModel_elem model2); assumption.
@@ -207,181 +154,30 @@ Lemma SuperModel_trans {flds1 sig1} (model1 : Model (flds:=flds1) sig1)
 Qed.
 
 
-(* FIXME: inductive version of SuperModel, plus (attempts!) at proofs *)
-(*
-Inductive SuperModel {flds1 sig1} (model1 : Model (flds:=flds1) sig1) :
-  forall {flds2 sig2}, Model (flds:=flds2) sig2 -> Prop :=
-| SuperModel_Nil : SuperModel model1 Model_Nil
-| SuperModel_Cons f A a flds2 sig2 model2 :
-    ModelElem f A a model1 ->
-    SuperModel model1 model2 ->
-    SuperModel model1 (Model_Cons f A a flds2 sig2 model2)
-.
-
-Lemma SuperModel_cons_l f A a {flds1 sig1} model1 {flds2 sig2} model2 :
-  SuperModel model1 (flds2:=flds2) (sig2:=sig2) model2 ->
-  SuperModel (Model_Cons f A a flds1 sig1 model1) model2.
-  intro super; induction super.
-  apply SuperModel_Nil.
-  apply SuperModel_Cons;
-    [ apply ModelElem_Cons | ]; assumption.
-Qed.
-
-Lemma SuperModel_id {flds sig} model :
-  SuperModel (flds1:=flds) (sig1:=sig) model model.
-  induction model.
-  apply SuperModel_Nil.
-  apply SuperModel_Cons;
-    [ apply ModelElem_Base
-    | apply SuperModel_cons_l; assumption ].
-Qed.
-
-
-(*
-Lemma SuperModel_fst :
-  
-  SuperModel model1 (Model_Cons f A a flds2 sig2 model2)
-*)
-
-
-Lemma SuperModel_elem {flds2 sig2} (model2 : Model (flds:=flds2) sig2)
-      f A a (elem : ModelElem f A a model2)
-      {flds1 sig1} (model1 : Model (flds:=flds1) sig1) :
-  SuperModel model1 model2 ->
-  ModelElem f A a model1.
-  revert flds1 sig1 model1; induction elem; intros.
-
-
-  intro super; induction super.
-  intros; inversion H.
-  intros. inversion H0.
-
-
-
-Lemma SuperModel_elem 
-      {flds1 sig1} (model1 : Model (flds:=flds1) sig1)
-      {flds2 sig2} (model2 : Model (flds:=flds2) sig2) :
-  SuperModel model1 model2 ->
-  forall f A a (elem : ModelElem f A a model2),
-  ModelElem f A a model1.
-  intro super; induction super; intros.
-  inversion elem.
-  inversion elem.
-
-Lemma SuperModel_trans {flds1 sig1} (model1 : Model (flds:=flds1) sig1)
-      {flds2 sig2} (model2 : Model (flds:=flds2) sig2)
-      {flds3 sig3} (model3 : Model (flds:=flds3) sig3) :
-  SuperModel model1 model2 -> SuperModel model2 model3 ->
-  SuperModel model1 model3.
-  intros super12 super23;
-  revert flds1 sig1 model1 super12; induction super23; intros.
-  apply SuperModel_Nil.
-
-
-  revert flds3 sig3 model3 super23; induction super12; intros.
-  inversion super23.
-*)
-
-
-(* FIXME: old version based on modelProj *)
-(*
-Inductive SuperModel {flds1 sig1} (model1 : Model (flds:=flds1) sig1) :
-  forall {flds2 sig2}, Model (flds:=flds2) sig2 -> Prop :=
-| SuperModel_Nil : SuperModel model1 Model_Nil
-| SuperModel_Cons f in_pf flds2 sig2 model2 :
-    SuperModel model1 model2 ->
-    SuperModel model1
-               (Model_Cons f (projT1 (modelProj model1 f in_pf))
-                           (projT2 (modelProj model1 f in_pf))
-                           flds2 sig2 model2)
-.
-*)
-
-
-
-
 (**
  ** Mapping functions over structures
  **)
 
-Fixpoint sig_map (g : string -> string) {flds} (sig : Sig flds) : Sig (map g flds) :=
-  match sig in Sig flds return Sig (map g flds) with
-    | Sig_Nil => Sig_Nil
-    | Sig_Cons f A flds sig =>
-      Sig_Cons (g f) A (map g flds) (fun a => sig_map g (sig a))
-  end.
-
-Fixpoint model_map (g : string -> string) {flds sig}
-         (model : Model (flds:=flds) sig) :
-  Model (flds:=map g flds) (sig_map g sig) :=
-  match model in Model sig return Model (sig_map g sig) with
+Fixpoint model_map (g : string -> string) {flds} (model : Model (flds:=flds)) :
+  Model (flds:=map g flds) :=
+  match model in Model (flds:=flds) return Model (flds:=map g flds) with
     | Model_Nil => Model_Nil
-    | Model_Cons f A a flds sig model =>
-      Model_Cons (g f) A a (map g flds) (fun a' => sig_map g (sig a'))
-                 (model_map g model)
+    | Model_Cons f A a flds model =>
+      Model_Cons (g f) A a (map g flds) (model_map g model)
   end.
 
-Fixpoint spec_map (g : string -> string) {flds sig}
-         (spec : Spec (flds:=flds) sig) :
-  Spec (flds:=map g flds) (sig_map g sig) :=
-  match spec in Spec sig return Spec (sig_map g sig) with
+Fixpoint spec_map (g : string -> string) {flds} (spec : Spec (flds:=flds)) :
+  Spec (flds:=map g flds) :=
+  match spec in Spec (flds:=flds) return Spec (flds:=map g flds) with
     | Spec_Nil => Spec_Nil
-    | Spec_ConsNone f A flds sig spec =>
-      Spec_ConsNone (g f) A (map g flds) (fun a => sig_map g (sig a))
-                    (fun a => spec_map g (spec a))
-    | Spec_ConsSome f A a flds sig spec =>
-      Spec_ConsSome (g f) A a (map g flds) (fun a' => sig_map g (sig a'))
-                    (spec_map g spec)
+    | Spec_ConsNone f A flds spec =>
+      Spec_ConsNone (g f) A (map g flds) (fun a => spec_map g (spec a))
+    | Spec_ConsSome f A a flds spec =>
+      Spec_ConsSome (g f) A a (map g flds) (spec_map g spec)
   end.
-
-
-(* sig_map id is the identity *)
-(* FIXME: prove this or remove it *)
-(*
-Lemma sig_map_id {flds} (sig : Sig flds) :
-  existT Sig (map id flds) (sig_map id sig) = existT Sig flds sig.
-  induction sig.
-  reflexivity.
-  unfold map; fold (map id flds).
-  unfold sig_map; fold (sig_map id (flds:=flds)).
-  assert
-    (existT (fun fs => A -> Sig fs) (map id flds) (fun a => sig_map id (s a))
-     = existT _ flds s).
-  Focus 2.
-  replace
-    (existT Sig (id f :: map id flds)
-      (Sig_Cons (id f) A (map id flds) (fun a : A => sig_map id (s a))))
-  with
-    ((fun tuple =>
-        existT Sig (f :: projT1 tuple) (Sig_Cons f A (projT1 tuple) (projT2 tuple)))
-       (existT (fun fs => A -> Sig fs) (map id flds) (fun a => sig_map id (s a))));
-    [ rewrite H0; reflexivity | ].
-  reflexivity.
-
-  assert (s = eq_rect _ (fun fs => A -> Sig fs) (fun a => sig_map id (s a)) _ (map_id _)).
-  apply functional_extensionality.
-  intro x.
-  symmetry.
-
-  apply eq_sigT_snd.
-  apply (eq_sigT_snd (H x)).
-
-  Print eq_sigT_snd.
-  rewrite <- (eq_sigT_snd )
-
-  Check inj_pair2.
-*)
-
-
-(* FIXME: prove this or remove it *)
-(*
-Lemma sig_map_trans {flds} f1 f2 (sig : Sig flds) :
-  existT Sig _ (sig_map (fun x => f2 (f1 x)) sig)
-  = existT Sig _ (sig_map f2 (sig_map f1 sig)).
-*)
 
 (* ModelElem commutes with mapping *)
-Lemma ModelElem_map {flds sig} (model : Model (flds:=flds) sig) m f A a :
+Lemma ModelElem_map {flds} (model : Model (flds:=flds)) m f A a :
   ModelElem f A a model -> ModelElem (m f) A a (model_map m model).
   intro melem; induction melem.
   apply ModelElem_Base.
@@ -389,38 +185,26 @@ Lemma ModelElem_map {flds sig} (model : Model (flds:=flds) sig) m f A a :
 Qed.
 
 (* IsModel commutes with mapping *)
-Lemma IsModel_hom_map_commutes {flds sig} (g : string -> string)
-      (spec : Spec (flds:=flds) sig) (model : Model sig) :
-  IsModel_hom spec model ->
-  IsModel_hom (spec_map g spec) (model_map g model).
+Lemma IsModel_map_commutes {flds} (g : string -> string)
+      (spec : Spec (flds:=flds)) (model : Model) :
+  IsModel spec model ->
+  IsModel (spec_map g spec) (model_map g model).
   intro ism; induction ism.
-  apply IsModel_hom_Nil.
-  apply IsModel_hom_ConsNone; apply IHism.
-  apply IsModel_hom_ConsSome; apply IHism.
+  apply IsModel_Nil.
+  apply IsModel_ConsNone; apply IHism.
+  apply IsModel_ConsSome; apply IHism.
 Qed.
 
-(* IsModel commutes with mapping *)
-Lemma IsModel_het_map_commutes {flds sig_s} (g : string -> string)
-      (spec : Spec (flds:=flds) sig_s)
-      {sig_m} (model : Model (flds:=flds) sig_m) :
-  IsModel_het spec model ->
-  IsModel_het (spec_map g spec) (model_map g model).
-  intro ism; induction ism.
-  apply IsModel_het_Nil.
-  apply IsModel_het_ConsNone; apply IHism.
-  apply IsModel_het_ConsSome; apply IHism.
-Qed.
-
-Lemma SuperModel_map_id {flds sig} model :
-  SuperModel (flds1:=flds) (sig1:=sig) model (model_map id model).
+Lemma SuperModel_map_id {flds} model :
+  SuperModel (flds1:=flds) model (model_map id model).
   induction model.
   apply I.
   split; [ apply ModelElem_Base | apply SuperModel_cons_l; assumption ].
 Qed.
 
-Lemma SuperModel_map_trans {flds1 sig1} (model1 : Model (flds:=flds1) sig1)
-      {flds2 sig2} (model2 : Model (flds:=flds2) sig2)
-      {flds3 sig3} (model3 : Model (flds:=flds3) sig3)
+Lemma SuperModel_map_trans {flds1} (model1 : Model (flds:=flds1))
+      {flds2} (model2 : Model (flds:=flds2))
+      {flds3} (model3 : Model (flds:=flds3))
       m1 m2 :
   SuperModel model3 (model_map m2 model2) ->
   SuperModel model2 (model_map m1 model1) ->
@@ -437,55 +221,25 @@ Lemma SuperModel_map_trans {flds1 sig1} (model1 : Model (flds:=flds1) sig1)
   apply IHmodel1; assumption.
 Qed.
 
-(* FIXME: old approach of translating models... *)
-
-(* Models can be translated by "unapplying" a function on fields *)
-(* FIXME: can only translate when we know the projected type is preserved
-Fixpoint modelXlate {flds1 sig1} :
-  ({f | In f flds1} -> {f | In f flds2}) ->
-  forall {flds2 sig2},
-    Model (flds:=flds2) sig2 ->
-    Model (flds:=flds1) sig1 :=
-  match sig1 in Sig flds1
-        return
-        ({f | In f flds1} -> {f | In f flds2}) ->
-        forall {flds2 sig2},
-          Model (flds:=flds2) sig2 ->
-          Model (flds:=flds1) sig1
-  with
-    | Sig_Nil => Model_Nil
-    | Sig_Cons f A flds nodup sig =>
-      fun xlate flds2 sig2 model2 =>
-        Model_Cons f A 
-*)
-
-(*
-Inductive ModelXlates {flds2 sig2} (model2 : Model (flds:=flds2) sig2) :
-  forall {flds1 sig1},
-    Model (flds:=flds1) sig1 ->
-    ({f | In f flds1} -> {f | In f flds2}) -> Prop :=
-| ModelXlates_Nil : ModelXlates model2
-*)
-
 
 (**
  ** Morphisms
  **)
 
 (* A morphism maps a spec to one with a subset of the models *)
-Definition IsMorphism {flds1 sig1} (spec1 : Spec (flds:=flds1) sig1)
-           {flds2 sig2} (spec2 : Spec (flds:=flds2) sig2)
+Definition IsMorphism {flds1} (spec1 : Spec (flds:=flds1))
+           {flds2} (spec2 : Spec (flds:=flds2))
            (m : string -> string) :=
   forall model2,
-    IsModel_hom spec2 model2 ->
-    { model1 : _ & IsModel_hom spec1 model1 & SuperModel model2 (model_map m model1) }.
+    IsModel spec2 model2 ->
+    { model1 : _ & IsModel spec1 model1 & SuperModel model2 (model_map m model1) }.
 
-Definition Morphism {flds1 sig1} (spec1 : Spec (flds:=flds1) sig1)
-           {flds2 sig2} (spec2 : Spec (flds:=flds2) sig2) :=
+Definition Morphism {flds1} (spec1 : Spec (flds:=flds1))
+           {flds2} (spec2 : Spec (flds:=flds2)) :=
   { m : _ & IsMorphism spec1 spec2 m }.
 
-Definition mkMorphism {flds1 sig1} (spec1 : Spec (flds:=flds1) sig1)
-           {flds2 sig2} (spec2 : Spec (flds:=flds2) sig2)
+Definition mkMorphism {flds1} (spec1 : Spec (flds:=flds1))
+           {flds2} (spec2 : Spec (flds:=flds2))
            (m : string -> string)
            (ism : IsMorphism spec1 spec2 m) : Morphism spec1 spec2 :=
   existT _ m ism.
@@ -495,19 +249,19 @@ Definition mkMorphism {flds1 sig1} (spec1 : Spec (flds:=flds1) sig1)
  ** Morphisms as a category
  **)
 
-Lemma IsMorphism_id {flds sig} (spec : Spec (flds:=flds) sig) :
+Lemma IsMorphism_id {flds} (spec : Spec (flds:=flds)) :
   IsMorphism spec spec id.
   intros model ism;
   apply (existT2 _ _ model); [ assumption | apply SuperModel_map_id ].
 Qed.
 
-Definition mid {flds sig} spec :
-  Morphism (flds1:=flds) (sig1:=sig) spec (flds2:=flds) (sig2:=sig) spec :=
+Definition mid {flds} spec :
+  Morphism (flds1:=flds) spec (flds2:=flds) spec :=
   mkMorphism spec spec id (IsMorphism_id _).
 
-Lemma IsMorphism_trans {flds1 sig1} (spec1 : Spec (flds:=flds1) sig1)
-      {flds2 sig2} (spec2 : Spec (flds:=flds2) sig2)
-      {flds3 sig3} (spec3 : Spec (flds:=flds3) sig3)
+Lemma IsMorphism_trans {flds1} (spec1 : Spec (flds:=flds1))
+      {flds2} (spec2 : Spec (flds:=flds2))
+      {flds3} (spec3 : Spec (flds:=flds3))
       m1 m2 :
   IsMorphism spec1 spec2 m1 ->
   IsMorphism spec2 spec3 m2 ->
@@ -520,9 +274,9 @@ Lemma IsMorphism_trans {flds1 sig1} (spec1 : Spec (flds:=flds1) sig1)
   apply (SuperModel_map_trans _ model2); assumption.
 Qed.
 
-Definition mcompose {flds1 sig1} {spec1 : Spec (flds:=flds1) sig1}
-      {flds2 sig2} {spec2 : Spec (flds:=flds2) sig2}
-      {flds3 sig3} {spec3 : Spec (flds:=flds3) sig3}
+Definition mcompose {flds1} {spec1 : Spec (flds:=flds1)}
+      {flds2} {spec2 : Spec (flds:=flds2)}
+      {flds3} {spec3 : Spec (flds:=flds3)}
       (morph1 : Morphism spec1 spec2)
       (morph2 : Morphism spec2 spec3) : Morphism spec1 spec3 :=
   mkMorphism spec1 spec3 (fun x => (projT1 morph2) (projT1 morph1 x))
@@ -533,17 +287,17 @@ Definition mcompose {flds1 sig1} {spec1 : Spec (flds:=flds1) sig1}
  ** Syntax for specs and morphism
  **)
 
+(*
 FIXME HERE: figure out notations
 
-Bind Scope spec_scope with Spec.
 
 Notation "{| |}" := Spec_Nil (at level 80).
 (* Notation "{| spec |}" := spec : spec_scope. *)
 
-Notation "{|  f  :  A  :=  a ;  spec  |}" := (Spec_ConsSome f A a _ (fun _ => _) spec) (at level 80, f at level 99).
-Notation "{|  f  :  A  ;  x  ->  spec  |}" := (Spec_ConsNone f A _ _ (fun x => spec)) (at level 80, f at level 99, x at level 99).
+Notation "{|  f  :  A  :=  a ;  spec  |}" := (Spec_ConsSome f A a _ spec) (at level 0, f at level 99).
+Notation "{|  f  :  A  ;  x  ->  spec  |}" := (Spec_ConsNone f A _ (fun x => spec)) (at level 0, f at level 99, x at level 99).
 
-Eval compute in (Spec_ConsNone "f1" nat _ _ (fun f1 => Spec_ConsSome "f2" nat 0 _ (fun _ => Sig_Nil) Spec_Nil)).
+Eval compute in (Spec_ConsNone "f1" nat _ (fun f1 => Spec_ConsSome "f2" nat 0 _ Spec_Nil)).
 
 Eval compute in ({| "f2" : nat := 0; {| |} |}).
 
@@ -552,3 +306,4 @@ Eval compute in ({| "f1" : nat ; f1 -> "f2" : nat := 0; {| |} |}).
 
 
 Eval compute in (Spec_ConsNone "f1" nat _ _ (fun f1 => Spec_ConsSome "f2" nat 0 _ (fun _ => Sig_Nil) Spec_Nil)).
+*)
